slides/README.md
@@ -1,0 +1,137 @@
+---
+title: Abstract Reachability
+subtitle: a semantics-based approach
+author: Traian Florin Șerbănuță (joint work with Virgil Șerbănuță and Dorel Lucanu)
+institute: Runtime Verification
+bibliography: k.bib
+theme: RV
+aspectratio: 169
+---
+
+## Motivation for this research
+
+- Algorithm for Reachability Logic Deduction for K
+  + with Virgil Șerbănuță and Xiaohong Chen
+- Idea to replace circular coinduction with regular induction
+  + to allow proving total correctness
+- I like formalizing mathematics with interactive provers
+  + I don't trust my math technical skills anymore
+- Fomalizing semantical notions is (a bit) easier
+
+## Results (so far)
+
+- Formalization of transition systems and traces
+- EF (exists finally) and AF (always finally) as fixpoints
+- A (semantics) deduction system for the intersection between CTL and Reachability Logic
+- Initial work on incorporating quantification
+
+# Preliminaries
+
+## Reachability Logic
+
+- Program verification logic for K [@rl-original]
+- Derives statements of the form $\varphi \Rightarrow \psi$
+- Two flavors: one-path and all-paths
+
+### One-path Reachability Logic [@rl-one-path]
+
+Whenever starting in a configuration matching $\varphi$ there is always an execution
+path leading to a configuration matching $\psi$
+
+### All-paths Reachability Logic [@rl-all-paths]
+
+A configuration matching $\psi$ will be reached on any execution path starting
+in a configuration matching $\varphi$.
+
+## Reachability Logic and CTL
+
+### Resemblance
+
+- one-path reachability formula: $\varphi \implies \mathop{EF} \psi$
+- all-paths reachability formula: $\varphi \implies \mathop{AF} \psi$
+
+### Differences
+
+- CTL is richer
+  + more temporal operators (AG, EG, AU, EU, ...)
+- Reachability Logic is richer
+  + Reachability formulae have structure and free variables
+
+## Matching Logic is the best!
+
+### Reachability Logic is richer than CTL
+- Reachability formulae have structure and constraints
+
+### Solution: Enter Matching Logic
+- A logic mixing patterns and constraints
+- Specifically designed to express matching for K
+- Fixed-point operators ($\mu$, $\nu$) introduced to capture reachability
+- Formulae interpreted as sets
+
+# Technical preliminaries
+
+## Transition systems and traces
+
+- A transition system is a set $D$ with a relation $\tau$ on it
+- $a \in D$ is _reducible_ iff $\exists b, a \mathrel{\tau} b$
+- A _transition sequence_ from $a$ to $b$ is 
+  + a (finite) non-empty sequence of elements from $D$
+  + such that any two consecutive elements are in relation $\tau$
+  + its first element is $a$ and its last element is $b$ (can be equal)
+- A _complete transition chain_ is
+  + a (possibly infinite) non-empty sequence of elements from $D$
+  + such that any two consecutive elements are in relation $\tau$
+  + and the final element (if there is one) is irreducible
+- the first element in a transition sequence/complete transition chain
+  is called the _head_
+
+## A set semantics for (a fragment) of CTL
+
+- $\mathop{EX} B = \{ a \mid \exists b \in B, a \mathrel{\tau} b \}$ 
+- $\mathop{AX} B = \complement{\left(\mathop{EX}{\left(\complement{B}\right)}\right)}$
+- $\mathop{EF} B = \{ a \mid t \textit{ transition system from } a \textit{ to } b \textit{ and } b \in B \}$
+- $\mathop{AF} B = \{ a \mid \forall t \textit{ complete transition chain}, \mathop{head} t = a \implies \exists b \in t, b \in B \}$
+
+## Exists-finally and Always-finally as fixed-points
+
+### Exists-finally
+
+- $\mathop{EF} \psi$ is the least-fixed-point of the functor
+$$F_{\mathop{EF}}(X) = \psi \cup \{ a \mid \exists b \in X, a \mathrel{\tau} b \}$$
+
+### Always-finally
+
+- $\mathop{AF} \psi$ is the least-fixed-point of the functor
+$$F_{\mathop{AF}}(X) = \psi \cup \{ a \mid \mathop{reducible} a \wedge \forall b, a \mathrel{\tau} b \implies b \in X \}$$
+
+# Deduction Rules
+
+## Deduction Rules for a relation $R$
+
+Rule of Reflexivity
+
+: $\displaystyle\frac{\checkmark }{\varphi \mathrel{R} \varphi}$
+
+Rule of Transitivity
+
+: $\displaystyle\frac{\varphi \mathrel{R} \psi \hspace{1em} \psi \mathrel{R} \chi}{\varphi \mathrel{R} \chi}$
+
+Rule of Consequence
+
+: $\displaystyle\frac{\varphi' \subseteq \varphi \hspace{1em} \varphi \mathrel{R} \psi \hspace{1em} \psi \subseteq \psi'}{\varphi' \mathrel{R} \psi'}$
+
+## Deduction Rules for a relation $R$
+
+Rule of Disjunction
+
+: $\displaystyle\frac{\varphi_1 \mathrel{R} \psi \hspace{1em} \varphi_2 \mathrel{R} \psi}{\varphi_1 \cup \varphi_2 \mathrel{R} \psi}$
+
+Rule of Generalization
+
+: $\displaystyle\frac{\varphi_i \mathrel{R} \psi \textrm{for all } i \in I}{\bigcup_{i\in I}\varphi_i \mathrel{R} \psi}$
+
+## Deduction Rules for a relation $R$
+
+
+
+## References
